Tutorial progress

book/LowStar.fst
@@ -1,5 +1,7 @@
 module LowStar
 
+module B = FStar.Buffer
+
 open FStar.HyperStack.ST
 
 /// The Low* subset of F*
@@ -11,14 +13,30 @@ open FStar.HyperStack.ST
 /// Low*, as formalized and presented on `paper <https://arxiv.org/abs/1703.00053>`_,
 /// is the first-order lambda calculus. Base types are booleans and
 /// fixed-width integers. Low* has a primitive notion of *buffers* and pointer
-/// arithmetic within buffer bounds.
+/// arithmetic within buffer bounds. In the formalization, structures are only
+/// valid when allocated within a buffer.
 ///
-/// These snippets are all valid Low* constructs.
+/// This section describes Low* by example, showing valid and invalid
+/// constructs, to give the reader a good grasp of what syntactic subset of the
+/// F* language constitutes valid Low*.
+///
+/// **These snippets are all valid Low* constructs.**
 
+// Supported: base types are machine integers, arithmetic is permitted
 let square (x: UInt32.t): UInt32.t =
   let open FStar.UInt32 in
   x *%^ x
 
+/// .. code:: c
+///
+///    uint32_t square(uint32_t x)
+///    {
+///      return x * x;
+///    }
+///
+/// .. fst::
+
+// Supported: classic control-flow
 let abs (x: Int32.t): Pure Int32.t
   (requires Int32.v x <> Int.min_int 32)
   (ensures fun r -> Int32.v r >= 0)
@@ -29,26 +47,167 @@ let abs (x: Int32.t): Pure Int32.t
   else
     0l -^ x
 
-/// These snippets are extensions to Low* (described in ??).
+/// .. code:: c
+///
+///    int32_t abs(int32_t x)
+///    {
+///      if (x >= (int32_t)0)
+///        return x;
+///      else
+///        return (int32_t)0 - x;
+///    }
+///
+/// .. fst::
 
-let min_int32 = FStar.Int32.(0l -^ 0x7fffffffl -^ 1l)
+// Supported: stack allocation
+let on_the_stack (): Stack UInt64.t (fun _ -> True) (fun _ _ _ -> True) =
+  let open B in
+  push_frame ();
+  let b = B.create 0UL 64ul in
+  b.(0ul) <- 32UL;
+  let r = b.(0ul) in
+  pop_frame ();
+  r
 
+/// .. code:: c
+///
+///    uint64_t on_the_stack()
+///    {
+///      uint64_t b[64U] = { 0U };
+///      b[0U] = (uint64_t)32U;
+///      uint64_t r = b[0U];
+///      return r;
+///    }
+///
+/// .. fst::
 
-// Extension: compiling F* inductives as structures passed by value in C
+// Supported: heap allocation
+let on_the_heap (): St UInt64.t =
+  let open B in
+  let b = B.rcreate_mm HyperStack.root 0UL 64ul in
+  b.(0ul) <- 32UL;
+  let r = b.(0ul) in
+  B.rfree b;
+  r
+
+/// .. code:: c
+///
+///    uint64_t on_the_heap()
+///    {
+///      uint64_t *b = KRML_HOST_CALLOC((uint32_t)64U, sizeof (uint64_t));
+///      b[0U] = (uint64_t)32U;
+///      uint64_t r = b[0U];
+///      KRML_HOST_FREE(b);
+///      return r;
+///    }
+///
+/// .. fst::
+
+// Supported: defining a non-parameterized record made of Low* types
 type uint128 = {
   low: UInt64.t;
   high: UInt64.t
 }
 
-// Extension: F*'s structural equality is compiled to a C function
+/// .. code:: c
+///
+///    typedef struct uint128_s
+///    {
+///      uint64_t low;
+///      uint64_t high;
+///    }
+///    uint128;
+///
+/// .. fst::
+
+// Supported: records in buffers
+let uint128_alloc (h l: UInt64.t): St (B.buffer uint128) =
+  Buffer.rcreate_mm HyperStack.root ({ low = l; high = h }) 1ul
+
+/// .. code:: c
+/// 
+///    uint128 *uint128_alloc(uint64_t h, uint64_t l)
+///    {
+///      KRML_CHECK_SIZE(sizeof (uint128), (uint32_t)1U);
+///      uint128 *buf = KRML_HOST_MALLOC(sizeof (uint128));
+///      buf[0U] = ((uint128){ .low = l, .high = h });
+///      return buf;
+///    }
+///
+/// .. fst::
+
+// Supported: path access for records in buffers
+let uint128_high (x: B.buffer uint128): Stack UInt64.t
+  (requires fun h -> B.live h x /\ B.length x = 1)
+  (ensures fun h0 _ h1 -> B.live h1 x)
+=
+  let open B in
+  (x.(0ul)).high
+
+/// .. code:: c
+///
+///    uint64_t uint128_high(uint128 *x)
+///    {
+///      return x->high;
+///    }
+///
+/// .. fst::
+
+// Supported: definition of global constants that evaluate to C constants, i.e.
+// arithmetic over numerical constants, see the C11 standard for what exactly is
+// allowed to be a constant.
+let min_int32 = FStar.Int32.(0l -^ 0x7fffffffl -^ 1l)
+
+/// .. code:: c
+///
+///    // Meta-evaluated by F*
+///    int32_t min_int32 = (int32_t)-2147483648;
+
+/// **These snippets are extensions to Low* (described in ??).**
+
+// Extensions:
+// - F*'s structural equality is compiled to a recursive C function
+// - x and y are structures that are passed by value in C; this has performance
+//   implications (see ??)
 let uint128_equal (x y: uint128) =
   x = y
+
+/// .. code:: c
+///
+///    static bool __eq__LowStar_uint128(uint128 y, uint128 x)
+///    {
+///      return true && x.low == y.low && x.high == y.high;
+///    }
+///    
+///    bool uint128_equal(uint128 x, uint128 y)
+///    {
+///      return __eq__LowStar_uint128(x, y);
+///    }
+///
+/// .. fst::
 
 // Extension: compiling F* inductives as tagged unions in C
 noeq
 type key =
   | Algorithm1: Buffer.buffer UInt32.t -> key
   | Algorithm2: Buffer.buffer UInt64.t -> key
+
+/// .. code:: c
+///
+///    typedef enum { Algorithm1, Algorithm2 } key_tags;
+///    
+///    typedef struct key_s
+///    {
+///      key_tags tag;
+///      union {
+///        uint32_t *case_Algorithm1;
+///        uint64_t *case_Algorithm2;
+///      }
+///      ;
+///    }
+///    key;
+///
+/// .. fst::
 
 // Extension: monomorphization of the option type
 let abs2 (x: Int32.t): option Int32.t =
@@ -60,6 +219,38 @@ let abs2 (x: Int32.t): option Int32.t =
   else
     Some (0l -^ x)
 
+/// .. code:: c
+///
+///    typedef enum { FStar_Pervasives_Native_None, FStar_Pervasives_Native_Some }
+///    FStar_Pervasives_Native_option__int32_t_tags;
+///    
+///    typedef struct FStar_Pervasives_Native_option__int32_t_s
+///    {
+///      FStar_Pervasives_Native_option__int32_t_tags tag;
+///      int32_t v;
+///    }
+///    FStar_Pervasives_Native_option__int32_t;
+///    
+///    FStar_Pervasives_Native_option__int32_t abs2(int32_t x)
+///    {
+///      if (x == min_int32)
+///        return ((FStar_Pervasives_Native_option__int32_t){ .tag = FStar_Pervasives_Native_None });
+///      else if (x >= (int32_t)0)
+///        return
+///          ((FStar_Pervasives_Native_option__int32_t){ .tag = FStar_Pervasives_Native_Some, .v = x });
+///      else
+///        return
+///          (
+///            (FStar_Pervasives_Native_option__int32_t){
+///              .tag = FStar_Pervasives_Native_Some,
+///              .v = (int32_t)0 - x
+///            }
+///          );
+///    }
+///
+/// .. fst::
+
+
 // Extension: compilation of pattern matches
 let fail_if #a #b (package: a * (a -> option b)): St b =
   let open C.Failure in
@@ -69,28 +260,217 @@ let fail_if #a #b (package: a * (a -> option b)): St b =
   | None -> failwith !$"invalid argument: fail_if"
   | Some x -> x
 
-// Extension: passing function pointers, monomorphization of tuple types as structs passed by value
+/// .. code:: c
+///
+///    int32_t
+///    fail_if__int32_t_int32_t(
+///      K___int32_t_int32_t____FStar_Pervasives_Native_option__int32_t package
+///    )
+///    {
+///      int32_t x = package.fst;
+///      FStar_Pervasives_Native_option__int32_t (*f)(int32_t x0) = package.snd;
+///      FStar_Pervasives_Native_option__int32_t scrut = f(x);
+///      if (scrut.tag == FStar_Pervasives_Native_None)
+///        return C_Failure_failwith__int32_t("invalid argument: fail_if");
+///      else if (scrut.tag == FStar_Pervasives_Native_Some)
+///      {
+///        int32_t x1 = scrut.v;
+///        return x1;
+///      }
+///      else
+///      {
+///        KRML_HOST_PRINTF("KreMLin abort at %s:%d\n%s\n",
+///          __FILE__,
+///          __LINE__,
+///          "unreachable (pattern matches are exhaustive in F*)");
+///        KRML_HOST_EXIT(255U);
+///      }
+///    }
+///
+/// .. fst::
+
+// Extension: passing function pointers, monomorphization of tuple types as
+// structs passed by value
 let abs3 (x: Int32.t): St Int32.t =
   fail_if (x, abs2)
 
-/// These snippets are not Low*.
+/// .. code:: c
+///
+///    int32_t abs3(int32_t x)
+///    {
+///      return
+///        fail_if__int32_t_int32_t((
+///            (K___int32_t_int32_t____FStar_Pervasives_Native_option__int32_t){ .fst = x, .snd = abs2 }
+///          ));
+///    }
+///
+/// .. fst::
 
-// Cannot be compiled: closure; solution: hoist the closure to a top-level function
+
+// Extension: use meta-programming in F* to reduce local closures
 let pow4 (x: UInt32.t): UInt32.t =
   let open FStar.UInt32 in
+  [@ inline_let ]
   let pow2 (y: UInt32.t) = y *%^ y in
   pow2 (pow2 x)
 
-// Cannot be compiled: polymorphic assume val; solution: make the function monomorphic, or provide a C macro
+/// .. code:: c
+///
+///    uint32_t pow4(uint32_t x)
+///    {
+///      uint32_t x0 = x * x;
+///      return x0 * x0;
+///    }
+///
+/// .. fst::
+
+// Extension: definition of a global that does not compile to a C constant
+let uint128_zero (): Tot uint128 =
+  { high = 0UL; low = 0UL }
+
+let zero = uint128_zero ()
+
+/// .. code:: bash
+///
+///    $ krml -skip-linking -no-prefix LowStar LowStar.fst
+///    (...)
+///    Warning 9: : Some globals did not compile to C values and must be
+///    initialized before starting main(). You did not provide a main function,
+///    so users of your library MUST MAKE SURE they call kremlinit_globals();
+///    (see kremlinit.c).
+///
+///    $ cat kremlinit.c
+///    (...)
+///    void kremlinit_globals()
+///    {
+///      zero = uint128_zero();
+///    }
+
+/// **These snippets are not Low*.**
+
+// Cannot be compiled:
+// - local recursive let-bindings are not Low*;
+// - local closure captures variable in scope (KreMLin does not do closure conversion)
+// - the list type is not Low*
+let filter_map #a #b (f: a -> option b) (l: list a): list b =
+  let rec aux (acc: list b) (l: list a): Tot (list b) (decreases l) =
+    match l with
+    | hd :: tl ->
+        begin match f hd with
+        | Some x -> aux (x :: acc) tl
+        | None -> aux acc tl
+        end
+    | [] ->
+        List.rev acc
+  in
+  aux [] l
+
+/// Trying to compile the snippet above will generate a warning when calling F*
+/// to generate a ``.krml`` file.
+///
+/// .. code:: bash
+///
+///    $ krml -skip-compilation -verbose LowStar.fst
+///    ⚙ KreMLin auto-detecting tools.
+///    (...)
+///    ✔ [F*,extract]
+///    <dummy>(0,0-0,0): (Warning 250) Error while extracting LowStar.filter_map
+///    to KreMLin (Failure("Internal error: name not found aux\n"))
+///
+/// .. fst::
+
+// Cannot be compiled: data types are compiled as flat structures in C, meaning
+// that the list type would have infinite size in C. This is compiled by KreMLin
+// but rejected by the C compiler. See ?? for an example of a linked list.
+type list_int32 =
+| Nil: list_int32
+| Cons: hd:Int32.t -> tl:list_int32 -> list_int32
+
+let mk_list (): St list_int32 =
+  Cons 0l Nil
+
+/// Trying to compile the snippet above will generate an error when calling the
+/// C compiler to generate a ``.o`` file.
+/// 
+/// .. code:: bash
+///
+///    $ krml -skip-linking -verbose LowStar.fst
+///    ⚙ KreMLin auto-detecting tools.
+///    (...)
+///    ✘ [CC,./LowStar.c]
+///    In file included from ./LowStar.c:8:0:
+///    ./LowStar.h:95:22: error: field ‘tl’ has incomplete type
+///       LowStar_list_int32 tl;
+///
+/// .. fst::
+
+
+// Cannot be compiled: polymorphic assume val; solution: make the function
+// monomorphic, or provide a C macro
 assume val pair_up: #a:Type -> #b:Type -> a -> b -> a * b
 
-// Cannot be compiled: an untagged union over types that are non-pointers; see section ?? for an unofficial KreMLin extension, or rewrite your code to use a data type
+/// Trying to compile the snippet above will generate a warning when calling F*
+/// to generate a ``.krml`` file.
+///
+/// .. code:: bash
+///
+///    $ krml -skip-compilation -verbose LowStar.fst
+///    ⚙ KreMLin auto-detecting tools.
+///    (...)
+///    ✔ [F*,extract]
+///    Not extracting LowStar.pair_up to KreMLin (polymorphic assumes are not supported)
+///
+/// .. fst::
+
+// Cannot be compiled: indexed types. See section ?? for an unofficial KreMLin
+// extension that works in some very narrow cases, or rewrite your code to make
+// t an inductive. KreMLin currently does not have support for untagged unions,
+// i.e. automatically making `t` a C union.
 type alg = | Alg1 | Alg2
-let key' (a: alg) =
+let t (a: alg) =
   match a with
-  | Alg1 -> Buffer.buffer UInt32.t
-  | Alg2 -> Buffer.buffer UInt64.t
-  
+  | Alg1 -> UInt32.t
+  | Alg2 -> uint128
+
+let default_t (a: alg): t a =
+  match a with
+  | Alg1 -> 0ul
+  | Alg2 -> zero
+
+/// Trying to compile the snippet above will generate invalid C code.
+///
+/// .. code:: c
+///
+///    void *default_t(alg a)
+///    {
+///      switch (a)
+///      {
+///        case Alg1:
+///          {
+///            return (void *)(uint32_t)0U;
+///          }
+///        case Alg2:
+///          {
+///            return (void *)zero
+///          }
+///        default:
+///          {
+///            KRML_HOST_PRINTF("KreMLin incomplete match at %s:%d\n", __FILE__, __LINE__);
+///            KRML_HOST_EXIT(253U);
+///          }
+///      }
+///    }
+///
+/// If you are lucky, the C compiler may generate an error:
+///
+/// .. code:: bash
+///
+///    $ krml -skip-linking LowStar.fst -add-include '"kremstr.h"' -no-prefix LowStar -warn-error +9
+///
+///    ✘ [CC,./LowStar.c]
+///    ./LowStar.c: In function ‘default_t’:
+///    ./LowStar.c:291:9: error: cannot convert to a pointer type
+///             return (void *)zero;
 ///
 /// .. _memory-model:
 ///
